nola/examples/rust_halt/mod.v
@@ -9,18 +9,25 @@ Section ty_mod.
     !rust_haltC CON, !rust_haltJ CON JUDG Σ}.
 
   (** [ty_mod]: Modification type *)
+  Definition ty'_mod_def {X Y} (f : Y → X) (T : ty CON Σ X) : ty' CON Σ Y :=
+    (λ t d yπ vl, ty_own T t d (f ∘ yπ) vl,
+      λ t d l α yπ, ty_shr T t d l α (f ∘ yπ)).
+  Lemma ty'_mod_aux : seal (@ty'_mod_def). Proof. by eexists _. Qed.
+  Definition ty'_mod {X Y} := ty'_mod_aux.(unseal) X Y.
+  Lemma ty'_mod_unseal : @ty'_mod = @ty'_mod_def.
+  Proof. by exact: seal_eq. Qed.
   Definition ty_mod {X Y} (f : Y → X) (T : ty CON Σ X) : ty CON Σ Y :=
-    pair (ty_size T)
-      (λ t d yπ vl, ty_own T t d (f ∘ yπ) vl,
-        λ t d l α yπ, ty_shr T t d l α (f ∘ yπ)).
+    (ty_size T, ty'_mod f T).
+  Lemma ty_mod_unseal : @ty_mod = λ _ _ f T, (ty_size T, ty'_mod_def f T).
+  Proof. by rewrite /ty_mod ty'_mod_unseal. Qed.
 
   Context {X Y} {f : X → Y}.
 
   (** [ty_mod] is size-preserving *)
   #[export] Instance ty_mod_preserv : Preserv (@ty_mod _ _ f).
   Proof.
-    move=> ??? /ty_proeqv[?[eqvO eqvS]]. apply ty_proeqv=>/=. split; [done|].
-    split=> >; [exact: eqvO|exact: eqvS].
+    move=> ??? /ty_proeqv[?[eqvO eqvS]]. rewrite ty_mod_unseal.
+    apply ty_proeqv=>/=. split; [done|]. split=> >; [exact: eqvO|exact: eqvS].
   Qed.
   #[export] Instance ty_mod_proper : Proper ((≡) ==> (≡)) (@ty_mod _ _ f).
   Proof. apply preserv_proper, _. Qed.
@@ -34,8 +41,8 @@ Section ty_mod.
   (** [ty_mod] preserves [Ty] *)
   #[export] Instance ty_mod_ty `{!Ty T} : Ty (ty_mod f T).
   Proof.
-    split=>/= >. { exact _. } { exact: ty_own_size. }
-    { exact: ty_own_depth. } { exact: ty_shr_depth. }
+    rewrite ty_mod_unseal. split=>/= >. { exact _. }
+    { exact: ty_own_size. } { exact: ty_own_depth. } { exact: ty_shr_depth. }
     { move=> eq. apply: ty_own_clair=>/= ?. by rewrite eq. }
     { move=> eq. apply: ty_shr_clair=>/= ?. by rewrite eq. }
   Qed.
@@ -44,7 +51,7 @@ Section ty_mod.
   #[export] Instance ty_mod_ty_op `(!TyOpAt T κ d, !Inj (=) (=) f) :
     TyOpAt (ty_mod f T) κ d.
   Proof.
-    split=>/= >.
+    rewrite ty_mod_unseal. split=>/= >.
     - iIntros "κ T". iMod (ty_own_proph with "κ T") as (???) "[$$]".
       iPureIntro. by eapply proph_dep_unf.
     - iIntros "κα T". iMod (ty_shr_proph with "κα T") as (???) "[$$]".
@@ -54,21 +61,25 @@ Section ty_mod.
 
   (** [ty_mod] preserves [Send] *)
   #[export] Instance ty_mod_send `{!Send T} : Send (ty_mod f T).
-  Proof. move=>/= >. exact: send. Qed.
+  Proof. rewrite ty_mod_unseal. move=>/= >. exact: send. Qed.
   (** [ty_mod] preserves [Sync] *)
   #[export] Instance ty_mod_sync `{!Sync T} : Sync (ty_mod f T).
-  Proof. move=>/= >. exact: sync. Qed.
+  Proof. rewrite ty_mod_unseal. move=>/= >. exact: sync. Qed.
   (** [ty_mod] preserves [Copy] *)
   #[export] Instance ty_mod_copy `{!Copy T} : Copy (ty_mod f T).
-  Proof. split=>/= >; [exact _|exact: copy_shr_acc]. Qed.
+  Proof.
+    rewrite ty_mod_unseal. split=>/= >; [exact _|exact: copy_shr_acc].
+  Qed.
 
   (** Subtyping on [ty_mod] *)
   Lemma subty_of_mod {δ T} : ⊢ subty δ (ty_mod f T) T f.
-  Proof. rewrite subty_unseal. iSplit; iModIntro; by iIntros. Qed.
+  Proof.
+    rewrite subty_unseal ty_mod_unseal. iSplit; iModIntro; by iIntros.
+  Qed.
   Lemma subty_to_mod {δ g} `{!Ty T} :
     (∀ x, f (g x) = x) → ⊢ subty δ T (ty_mod f T) g.
   Proof.
-    rewrite subty_unseal=> eq. iSplit; iModIntro=>/=.
+    rewrite subty_unseal ty_mod_unseal=> eq. iSplit; iModIntro=>/=.
     - iIntros (????) "T". iApply (ty_own_clair with "T")=>//=.
     - iIntros (?????) "T". iApply (ty_shr_clair with "T")=>//=.
   Qed.
@@ -76,5 +87,5 @@ Section ty_mod.
   (** Resolution over [ty_mod] *)
   #[export] Instance resol_mod `(!ResolAt T κ post d) :
     ResolAt (ty_mod f T) κ (post ∘ f) d.
-  Proof. split=> > /=. exact: resol. Qed.
+  Proof. rewrite ty_mod_unseal. split=> > /=. exact: resol. Qed.
 End ty_mod.
